%
% This document provides a single place for definitions
% that will appear in multiple locations,
% and so ensures they are kept consistent.
%
% This does not generate any typeset output.
%
\def\LNAME#1{\mbox{\textsc{#1}}}
\def\QNAME#1{\LNAME{``{#1}''}}



%%%%  ==== Substitutions ========================================================

\def\DEFOEESUBST{
  \begin{eqnarray*}
     k[\vec x:=\vec e] &\defs& k
  \\ x[\vec x:=\vec e]
     &\defs& \left\{
               \begin{array}{ll}
                 e_i, & i \mbox{ exists, s.t.: }x=x_i \\
                 x, & x \notin \vec x
               \end{array}
             \right.
  \\ (f~e)[\vec x:=\vec e] &\defs& f~(e[\vec x:=\vec e])
  \\ E[\vec x:=\vec e] &\defs&
     \left\{
     \begin{array}{ll}
       E[\vec e/\vec x], & E \mbox{ not $\Lambda$-bound higher up} \\
       E, & E \mbox{ is $\Lambda$-bound higher up}
     \end{array}
   \right.
  \\ (\lambda \vec y, \lstvec q @ e)[\vec x:=\vec e]
     &\defs& \lambda \vec y,\lstvec q @ (e[\vec x:=\vec e]\hide\vec y)
  \\ (\Lambda \vec E @ e)[\vec x:=\vec e] &\defs& \Lambda \vec E @ (e[\vec x:=\vec e])
  \\ (\Lambda \vec P @ e)[\vec x:=\vec e] &\defs& \Lambda \vec P @ (e[\vec x:=\vec e])
  \\ (e[\vec f/\vec y])[\vec x:=\vec e] &\defs& e([\vec f/\vec y][\vec e/\vec x])
  \\ (e[\vec e/\vec E])[\vec x:=\vec e] &\defs& \mbox{need to do inner subst first}
  \\ (e[\vec p/\vec P])[\vec x:=\vec e] &\defs& \mbox{need to do inner subst first}
  \\ (e = e)[\vec x:=\vec e] &\defs& e[\vec x:=\vec e] = e[\vec x:=\vec e]
  \\ (\theta x | P @ Q)[\vec x:=\vec e] &\defs& \theta x | P[\vec x:=\vec e]\hide x @ Q[\vec x:=\vec e]\hide x
  \end{eqnarray*}
}

\def\DEFOEPSUBST#1{
\begin{array}{rcl@{$\quad$}l}
   True[\vec x:=\vec e] &\defs&  True
\\ False[\vec x:=\vec e] &\defs& False
\\  e[\vec x:=\vec e] &\defs& \mbox{see Figure \ref{#1}}
\\  (e:t)[\vec x:=\vec e] &\defs& (e[\vec x:=\vec e]:t)
\\  (\mathcal D~e)[\vec x:=\vec e] &\defs& \mathcal D~(e[\vec x:=\vec e])
\\ (\lnot p)[\vec x:=\vec e] &\defs& \lnot (p[\vec x:=\vec e])
\\ (p~ \maltese q)[\vec x:=\vec e] &\defs& p[\vec x:=\vec e]~ \maltese q[\vec x:=\vec e]
\\ P[\vec x:=\vec e] &\defs&
   \left\{
     \begin{array}{ll}
       P[\vec e/\vec x], & P \mbox{ not $\Lambda$-bound higher up} \\
       P, & P \mbox{ is $\Lambda$-bound higher up}
     \end{array}
   \right.
\\ (\yen \vec y,\lstvec q | p @ q)[\vec x:=\vec e]
   &\defs& \yen \vec y,\lstvec q | (p[\vec x:=\vec e]\hide \vec y) @ (q[\vec x:=\vec e]\hide \vec y))
\\ (\yen \vec P @ p)[\vec x:=\vec e] &\defs& \yen \vec P @ (p[\vec x:=\vec e])
\\ (\yen \vec E @ p)[\vec x:=\vec e] &\defs& \yen \vec E @ (p[\vec x:=\vec e])
\\ {}[ p ][\vec x:=\vec e] &\defs& {}[p]
\\ (\Lambda \vec y,\lstvec q @ p)[\vec x:=\vec e]
   &\defs& \Lambda \vec y,\lstvec q @ (p[\vec x:=\vec e]\hide \vec y)
\\ (\Lambda \vec P @ p)[\vec x:=\vec e] &\defs& \Lambda \vec P @ (p[\vec x:=\vec e])
\\ (p~\lstvec q)[\vec x:=\vec e] &\defs& (p[\vec x:=\vec e] ~\lstvec q[\vec x:=\vec e] )
\\ (p~\vec f)[\vec x:=\vec e] &\defs& (p[\vec x:=\vec e]~\vec f[\vec x:=\vec e])
\\ (p[\vec f/\vec y])[\vec x:=\vec e] &\defs& p([\vec f/\vec y][\vec e/\vec x])
\\ (p[\vec e/\vec E])[\vec x:=\vec e] &\defs& \mbox{need to do inner subst first}
\\ (p[\vec p/\vec P])[\vec x:=\vec e] &\defs& \mbox{need to do inner subst first}
\\ (p~S)[\vec x:=\vec e] &\defs& p[\vec x:=\vec e]~S[\vec x:=\vec e]
\\ (p \in S)[\vec x:=\vec e] &\defs& p[\vec x:=\vec e] \in S[\vec x:=\vec e]
\\
\\ S[\vec x:=\vec e] &\defs& S[\vec e/\vec x]
\\ \{ \vec p \}[\vec x:=\vec e] &\defs& \{ \vec p[\vec x:=\vec e] \}
\\ \{ \vec P | r @ p \}[\vec x:=\vec e]
    &\defs& \{ \vec P | r[\vec x:=\vec e] @ p[\vec x:=\vec e] \}
\\ (ps_1 \bigcup ps_2)[\vec x:=\vec e] &\defs& ps_1[\vec x:=\vec e] \bigcup ps_2[\vec x:=\vec e]
\end{array}
}

\def\DEFEEESUBST{
  \begin{eqnarray*}
     k[\vec E:=\vec e] &\defs& k
  \\ x[\vec E:=\vec e] &\defs& x
    \\ (f~e)[\vec E:=\vec e] &\defs& f~(e[\vec E:=\vec e])
  \\ E[\vec E:=\vec e]
     &\defs& \left\{
               \begin{array}{ll}
                 e_i, & i \mbox{ exists, s.t.: }E=E_i \\
                 E, & E \notin \vec E
               \end{array}
             \right.
  \\ (\lambda \vec x, \lstvec q @ e)[\vec E:=\vec e]
     &\defs& \lambda \vec x,\lstvec q @ (e[\vec E:=\vec e])
  \\ (\Lambda \vec F @ e)[\vec E:=\vec e]
     &\defs& \Lambda \vec F @ (e[\vec E:=\vec e]\hide \vec F)
  \\ (\Lambda \vec P @ e)[\vec E:=\vec e] &\defs& \Lambda \vec P @ (e[\vec E:=\vec e])
  \\ (e[\vec e/\vec x])[\vec E:=\vec e] &\defs& \mbox{need to do inner subst first}
  \\ (e[\vec f\vec F])[\vec E:=\vec e] &\defs& e([\vec f/\vec F][\vec e/\vec E])
  \\ (e[\vec p/\vec P])[\vec E:=\vec e] &\defs& \mbox{need to do inner subst first}
  \\ (e = e)[\vec E:=\vec e] &\defs& e[\vec E:=\vec e] = e[\vec E:=\vec e]
  \\ (\theta x | P @ Q)[\vec E:=\vec e]
     &\defs& \theta x | P[\vec E:=\vec e] @ Q[\vec E:=\vec e]
  \end{eqnarray*}
}

\def\DEFPPESUBST{
  \begin{eqnarray*}
     k[\vec P:=\vec p] &\defs& k
  \\ x[\vec P:=\vec p] &\defs& x
    \\ (f~e)[\vec P:=\vec p] &\defs& f~(e[\vec P:=\vec p])
  \\ E[\vec P:=\vec p] &\defs&
  \left\{
     \begin{array}{ll}
       E[\vec p/\vec P], & E \mbox{ not $\Lambda$-bound higher up} \\
       E, & E \mbox{ is $\Lambda$-bound higher up}
     \end{array}
   \right.
    \\ (\lambda \vec x, \lstvec q @ e)[\vec P:=\vec p]
     &\defs& \lambda \vec x,\lstvec q @ (e[\vec P:=\vec p])
  \\ (\Lambda \vec F @ e)[\vec P:=\vec p]
     &\defs& \Lambda \vec F @ (e[\vec P:=\vec p]\hide \vec F)
  \\ (\Lambda \vec P @ e)[\vec P:=\vec p] &\defs& \Lambda \vec P @ (e[\vec P:=\vec p])
  \\ (e[\vec e/\vec x])[\vec P:=\vec p] &\defs& \mbox{need to do inner subst first}
  \\ (e[\vec e/\vec E])[\vec P:=\vec p] &\defs& \mbox{need to do inner subst first}
  \\ (e[\lstvec q/\vec Q])[\vec P:=\vec p] &\defs& e([\lstvec q/\vec Q][\vec p/\vec P])
  \\ (e = e)[\vec P:=\vec p] &\defs& e[\vec P:=\vec p] = e[\vec P:=\vec p]
  \\ (\theta x | P @ Q)[\vec P:=\vec p]
     &\defs& \theta x | P[\vec P:=\vec p] @ Q[\vec P:=\vec p]
  \end{eqnarray*}
}


\def\DEFEEPSUBST#1{
\begin{array}{rcl@{$\quad$}l}
   True[\vec E:=\vec e] &\defs&  True
\\ False[\vec E:=\vec e] &\defs& False
\\  e[\vec E:=\vec e] &\defs& \mbox{see Figure \ref{#1}}
\\  (e:t)[\vec E:=\vec e] &\defs& (e[\vec E:=\vec e]:t)
\\  (\mathcal D~e)[\vec E:=\vec e] &\defs& \mathcal D~(e[\vec E:=\vec e])
\\ (\lnot p)[\vec E:=\vec e] &\defs& \lnot (p[\vec E:=\vec e])
\\ (p~ \maltese q)[\vec E:=\vec e] &\defs& p[\vec E:=\vec e]~ \maltese q[\vec E:=\vec e]
\\ P[\vec E:=\vec e] &\defs&
   \left\{
     \begin{array}{ll}
       P[\vec e/\vec x], & P \mbox{ not $\Lambda$-bound higher up} \\
       P, & P \mbox{ is $\Lambda$-bound higher up}
     \end{array}
   \right.
\\ (\yen \vec y,\lstvec q | p @ q)[\vec E:=\vec e]
   &\defs& \yen \vec y,\lstvec q | (p[\vec E:=\vec e]) @ (q[\vec E:=\vec e]))
\\ (\yen \vec P @ p)[\vec E:=\vec e] &\defs& \yen \vec P @ (p[\vec E:=\vec e])
\\ (\yen \vec F @ p)[\vec E:=\vec e] &\defs& \yen \vec F @ (p[\vec E:=\vec e]\hide\vec F)
\\ {}[~p~][\vec E:=\vec e] &\defs& {}[~p[\vec E:=\vec e]~]
\\ (\Lambda \vec y,\lstvec q @ p)[\vec E:=\vec e]
   &\defs& \Lambda \vec y,\lstvec q @ (p[\vec E:=\vec e])
\\ (\Lambda \vec P @ p)[\vec E:=\vec e] &\defs& \Lambda \vec P @ (p[\vec E:=\vec e])
\\ (p~\lstvec q)[\vec E:=\vec e] &\defs& (p[\vec E:=\vec e] ~\lstvec q[\vec E:=\vec e] )
\\ (p~\vec f)[\vec E:=\vec e] &\defs& (p[\vec E:=\vec e]~\vec f[\vec E:=\vec e])
\\ (p[\vec f/\vec y])[\vec E:=\vec e] &\defs& \mbox{need to do inner subst first}
\\ (p[\vec e/\vec E])[\vec E:=\vec e] &\defs& p([\vec e/\vec E][\vec e/\vec E]
\\ (p[\vec p/\vec P])[\vec E:=\vec e] &\defs& \mbox{need to do inner subst first}
\\ (p~S)[\vec E:=\vec e] &\defs& p[\vec E:=\vec e]~S[\vec E:=\vec e]
\\ (p \in S)[\vec E:=\vec e] &\defs& p[\vec E:=\vec e] \in S[\vec E:=\vec e]
\\
\\ S[\vec E:=\vec e] &\defs& S[\vec e/\vec E]
\\ \{ \vec p \}[\vec E:=\vec e] &\defs& \{ \vec p[\vec E:=\vec e] \}
\\ \{ \vec P | r @ p \}[\vec E:=\vec e]
    &\defs& \{ \vec P | r[\vec E:=\vec e] @ p[\vec E:=\vec e] \}
\\ (ps_1 \bigcup ps_2)[\vec E:=\vec e] &\defs& ps_1[\vec E:=\vec e] \bigcup ps_2[\vec E:=\vec e]
\end{array}
}

\def\DEFPPPSUBST#1{
\begin{array}{rcl@{$\quad$}l}
   True[\vec P:=\vec p] &\defs&  True
\\ False[\vec P:=\vec p] &\defs& False
\\  e[\vec P:=\vec p] &\defs& \mbox{see Figure \ref{#1}}
\\  (e:t)[\vec P:=\vec p] &\defs& (e[\vec P:=\vec p]:t)
\\  (\mathcal D~e)[\vec P:=\vec p] &\defs& \mathcal D~(e[\vec P:=\vec p])
\\ (\lnot p)[\vec P:=\vec p] &\defs& \lnot (p[\vec P:=\vec p])
\\ (p~ \maltese q)[\vec P:=\vec p] &\defs& p[\vec P:=\vec p]~ \maltese q[\vec P:=\vec p]
\\ P[\vec P:=\vec p] &\defs&
   \left\{
               \begin{array}{ll}
                 p_i, & P \mbox{ not bound higher} \\
                      & \mbox{and exists $i$ s.t.: }P=P_i \\
                 P, & \mbox{otherwise}
               \end{array}
             \right.
\\ (\yen \vec y,\lstvec q | p @ q)[\vec P:=\vec p]
   &\defs& \yen \vec y,\lstvec q | (p[\vec P:=\vec p]) @ (q[\vec P:=\vec p]))
\\ (\yen \vec Q @ p)[\vec P:=\vec p] &\defs& \yen \vec Q @ (p[\vec P:=\vec p]\hide\vec Q)
\\ (\yen \vec F @ p)[\vec P:=\vec p] &\defs& \yen \vec F @ (p[\vec P:=\vec p])
\\ {}[~p~][\vec P:=\vec p] &\defs& {}[~p[\vec P:=\vec p]~]
\\ (\Lambda \vec y,\lstvec q @ p)[\vec P:=\vec p]
   &\defs& \Lambda \vec y,\lstvec q @ (p[\vec P:=\vec p])
\\ (\Lambda \vec Q @ p)[\vec P:=\vec p] &\defs& \Lambda \vec P @ (p[\vec P:=\vec p]\hide \vec Q)
\\ (p~\lstvec q)[\vec P:=\vec p] &\defs& (p[\vec P:=\vec p] ~\lstvec q[\vec P:=\vec p] )
\\ (p~\vec f)[\vec P:=\vec p] &\defs& (p[\vec P:=\vec p]~\vec f[\vec P:=\vec p])
\\ (p[\vec f/\vec y])[\vec P:=\vec p] &\defs& \mbox{need to do inner subst first}
\\ (p[\vec e/\vec E])[\vec P:=\vec p] &\defs& \mbox{need to do inner subst first}
\\ (p[\lstvec q/\vec Q])[\vec P:=\vec p] &\defs& (p([\lstvec q/\vec Q][\vec p/\vec P])
\\ (p~S)[\vec P:=\vec p] &\defs& p[\vec P:=\vec p]~S[\vec P:=\vec p]
\\ (p \in S)[\vec P:=\vec p] &\defs& p[\vec P:=\vec p] \in S[\vec P:=\vec p]
\\
\\ S[\vec P:=\vec p] &\defs& S[\vec p/\vec P]
\\ \{ \vec p \}[\vec P:=\vec p] &\defs& \{ \vec p[\vec P:=\vec p] \}
\\ \{ \vec Q | r @ p \}[\vec P:=\vec p]
    &\defs& \{ \vec P
             | r[\vec P:=\vec p]\hide\vec Q
             @ p[\vec P:=\vec p] \hide\vec Q
            \}
\\ (ps_1 \bigcup ps_2)[\vec P:=\vec p] &\defs& ps_1[\vec P:=\vec p] \bigcup ps_2[\vec P:=\vec p]
\end{array}
}




%%%%  ==== Propositions ========================================================

%% ---- Propositional Axioms ---------------------------------------------------

\def\AXtrue{\true}
\def\AXtrueN{\QNAME{$\true$}}

\def\AXeqvRefl{P \equiv P}
\def\AXeqvReflN{\QNAME{$\equiv$-refl}}

\def\CJeqvId{\true \equiv Q\equiv Q}
\def\CJeqvIdN{\QNAME{$\equiv$-id}}

\def\AXeqvAssocL{(P\equiv Q)\equiv R}
\def\AXeqvAssocR{P\equiv (Q\equiv R)}
\def\AXeqvAssoc{(\AXeqvAssocL) \equiv (\AXeqvAssocR)}
\def\AXeqvAssocN{\QNAME{$\equiv$-assoc}}

\def\AXeqvSymm{P\equiv Q\equiv Q \equiv P}
\def\AXeqvSymmN{\QNAME{$\equiv$-symm}}

\def\AXfalseDef{\false \equiv \neg \true}
\def\AXfalseDefN{\QNAME{$\false$-def}}

\def\AXnotEqvDistr{\neg(P\equiv Q) \equiv \neg P \equiv Q}
\def\AXnotEqvDistrN{\QNAME{$\neg$-$\equiv$-distr}}

\def\AXorSymm{P\vee Q \equiv  Q \vee P}
\def\AXorSymmN{\QNAME{$\vee$-symm}}

\def\AXorAssoc{(P\vee Q) \vee R \equiv  P \vee (Q \vee R)}
\def\AXorAssocN{\QNAME{$\vee$-assoc}}

\def\AXorIdem{P\vee P \equiv P}
\def\AXorIdemN{\QNAME{$\vee$-idem}}

\def\AXorEqvDistr{P \vee (Q\equiv R) \equiv P\vee Q \equiv P \vee R}
\def\AXorEqvDistrN{\QNAME{$\vee$-$\equiv$-distr}}

\def\AXexclMdl{P \vee \neg P}
\def\AXexclMdlN{\QNAME{Excl-Mdl}}

\def\AXgoldRule{P\wedge Q \equiv  P \equiv Q \equiv P \vee Q}
\def\AXgoldRuleN{\QNAME{Golden-Rule}}

\def\AXimplDef{P\Rightarrow Q \equiv P\vee  Q \equiv Q}
\def\AXimplDefN{\QNAME{$\implies$-def}}

\def\AXPROP{
  \begin{array}{ll}
     \AXtrue & \AXtrueN
  \\ \AXeqvRefl & \AXeqvReflN
  \\ \AXeqvAssoc & \AXeqvAssocN
  \\ \AXeqvSymm & \AXeqvSymmN
  \\ \AXfalseDef &\AXfalseDefN
  \\ \AXnotEqvDistr & \AXnotEqvDistrN
  \\ \AXorSymm & \AXorSymmN
  \\ \AXorAssoc & \AXorAssocN
  \\ \AXorIdem & \AXorIdemN
  \\ \AXorEqvDistr & \AXorEqvDistrN
  \\ \AXexclMdl & \AXexclMdlN
  \\ \AXgoldRule & \AXgoldRuleN
  \\ \AXimplDef & \AXimplDefN
  \end{array}
}


%% ---- Propositional Conjectures ----------------------------------------------

% -- Equivalence -----------------------

\def\CJeqvId{\textit{true} \equiv Q\equiv Q}
\def\CJeqvIdN{\QNAME{$\equiv$-id}}

\def\CONJPROPEQUIV{
  \begin{array}{ll}
       \CJeqvId & \CJeqvIdN
  \end{array}
}

% % Negation, inequivalence and FALSE

\def\CJswapNot{\lnot P\equiv Q \equiv P \equiv \lnot Q}
\def\CJswapNotN{\QNAME{$\lnot$-$\equiv$-swap}}

\def\CJnotInvol{\lnot \lnot P \equiv P}
\def\CJnotInvolN{\QNAME{$\lnot$-invol}}

\def\CJnotFalse{\lnot \false \equiv \true}
\def\CJnotFalseN{\QNAME{$\false$-neg}}

\def\CJnotDef{\lnot P \equiv P \equiv \false}
\def\CJnotDefN{\QNAME{$\lnot$-def}}

\def\CONJPROPNOT{
  \begin{array}{ll}
       \CJswapNot  & \CJswapNotN
    \\ \CJnotInvol & \CJnotInvolN
    \\ \CJnotFalse & \CJnotFalseN
    \\ \CJnotDef   & \CJnotDefN
  \end{array}
}

% \def\lawFalseDef{\NmCmtLaw{\m\FALSE-def}{$\GSN{3.8}$}{\FALSE \equiv \lnot \TRUE}}
% \def\lawNotEqvDistr{\NmCmtLaw{$\lnot$-$\equiv$-distr}{$\GSN{3.9}$}{\lnot(p\equiv q) \equiv \lnot p \equiv q}}
% \def\lawNEqvDef{\NmCmtLaw{$\not\equiv$-def}{$\GSN{3.10}$}{(p\not\equiv q) \equiv \lnot(p\equiv q)}}
% \def\lawNotEqvSwap{\NmCmtLaw{$\lnot$-$\equiv$-swap}{$\GSN{3.11}$}{\lnot p\equiv q \equiv p \equiv \lnot q}}
% \def\lawNotFalse{\NmCmtLaw{$\FALSE$-neg}{$\GSN{3.13}$}{\lnot \FALSE \equiv \TRUE}}
% \def\lawNEqvAlt{\NmCmtLaw{$\lnot$-$\equiv$-swap}{$\GSN{3.14}$}{(p\not \equiv q) \equiv \lnot p \equiv q}}
% \def\lawNEqvAAlt{\NmCmtLaw{$\not\equiv$-def}{$\GSN{3.15}$}{\lnot p \equiv p \equiv \FALSE}}
% \def\lawNEqvComm{\NmCmtLaw{$\not\equiv$-comm}{$\GSN{3.16}$}{(p\not \equiv q) \equiv (q\not\equiv p)}}
% \def\lawNEqvAssoc{\NmCmtLaw{$\not\equiv$-assoc}{$\GSN{3.17}$}{((p\not\equiv q)\not\equiv r) \equiv (p\not\equiv (q\not\equiv r))}}
% \def\lawNEqvMutual{\NmCmtLaw{$\not\equiv$-mutual}{$\GSN{3.18}$}{((p\not \equiv q)\equiv r) \equiv (p\not\equiv (q\equiv r))}}
% \def\lawNotEqvIntchg{\NmCmtLaw{$\not\equiv$-intchg}{$\GSN{3.19}$}{p\not \equiv q \equiv r\ \equiv\ p\equiv q\not \equiv r}}

% -- Disjunction -----------------------

\def\CJorZero{P \lor \textit{true} \equiv \textit{true}}
\def\CJorZeroN{\QNAME{$\lor$-zero}}

\def\CJorUnit{P \lor \textit{false} \equiv P}
\def\CJorUnitN{\QNAME{$\lor$-unit}}

\def\CJorDistr{P \lor (Q\lor R) \equiv (P\lor Q) \lor (P \lor R)}
\def\CJorDistrN{\QNAME{$\lor$-$\lor$-distr}}

\def\CJorEqvSplit{P\lor Q \equiv P \lor \lnot Q \equiv P}
\def\CJorEqvSplitN{\QNAME{$\lor$-$\equiv$-split}}

\def\CONJPROPDISJ{
  \begin{array}{ll}
       \CJorZero  & \CJorZeroN
    \\ \CJorUnit & \CJorUnitN
    \\ \CJorDistr & \CJorDistrN
    \\ \CJorEqvSplit & \CJorEqvSplitN
  \end{array}
}
% \def\lawOrZero{\NmCmtLaw{$\lor$-zero}{$\GSN{3.29}$}{p \lor \TRUE \equiv \TRUE}}
% \def\lawOrUnit{\NmCmtLaw{$\lor$-unit}{$\GSN{3.30}$}{p\lor \FALSE \equiv p}}
% \def\lawOrDistr{\NmCmtLaw{$\lor$-$\lor$-distr}{$\GSN{3.31}$}{p \lor (q\lor r) \equiv (p\lor q) \lor (p \lor r)}}
% \def\lawOrEqvSplit{\NmCmtLaw{$\lor$-$\equiv$-split}{$\GSN{3.32}$}{p\lor q \equiv p \lor \lnot q \equiv p}}
%
% % Conjunction
% \def\lawGldRule{\NmCmtLaw{golden-rule}{$\GSN{3.35}$}{p \land q \equiv p \equiv q \equiv p \lor q}}
% \def\lawAndComm{\NmCmtLaw{$\land$-comm}{$\GSN{3.36}$}{p\land q \equiv q \land p}}
% \def\lawAndAssoc{\NmCmtLaw{$\land$-assoc}{$\GSN{3.37}$}{(p\land q) \land r \equiv p \land (q \land r)}}
% \def\lawAndIdem{\NmCmtLaw{$\land$-idem}{$\GSN{3.38}$}{p\land p \equiv p}}
% \def\lawAndUnit{\NmCmtLaw{$\land$-unit}{$\GSN{3.39}$}{p\land \TRUE \equiv p}}
% \def\lawAndZero{\NmCmtLaw{$\land$-zero}{$\GSN{3.40}$}{p \land \FALSE \equiv \FALSE}}
% \def\lawAndDistr{\NmCmtLaw{$\land$-$\land$-distr}{$\GSN{3.41}$}{p \land (q\land r) \equiv (p\land q) \land (p \land r)}}
% \def\lawContradict{\NmCmtLaw{contradiction}{$\GSN{3.42}$}{p \land \lnot p \equiv \FALSE}}
%
% % Disj Conj
% \def\lawAndOrAbs{\NmCmtLaw{$\land$-$\lor$-absorb}{$\GSN{3.43}$}{p\land (p\lor q) \equiv p}}
% \def\lawOrAndAbs{\NmCmtLaw{$\lor$-$\land$-absorb}{$\GSN{3.43}$}{p \lor (p \land q) \equiv p}}
% \def\lawAndOrNAbs{\NmCmtLaw{$\land$-$\lor$-absorb}{$\GSN{3.44}$}{p \land (\lnot p\lor q) \equiv p \land q}}
% \def\lawOrAndNAbs{\NmCmtLaw{$\lor$-$\land$-absorb}{$\GSN{3.43}$}{p \lor (\lnot p \land q) \equiv p \lor q}}
% \def\lawOrAndDistr{\NmCmtLaw{$\lor$-$\land$-distr}{$\GSN{3.45}$}{p \lor (q\land r) \equiv (p\lor q) \land (p \lor r)}}
% \def\lawAndOrDistr{\NmCmtLaw{$\land$-$\lor$-distr}{$\GSN{3.46}$}{p \land (q\lor r) \equiv (p\land q) \lor (p \land r)}}
% \def\lawdeMorganNand{\NmCmtLaw{deMorgan}{$\GSN{3.47}$}{\lnot (p\land q) \equiv \lnot p \lor \lnot q}}
% \def\lawdeMorganNor{\NmCmtLaw{deMorgan}{$\GSN{3.47}$}{\lnot (p\lor q) \equiv \lnot p \land \lnot q}}
% \def\lawRepl{\NmCmtLaw{replacment}{$\GSN{3.51}$}{(p\equiv q) \land (r \equiv p) \equiv (p\equiv q) \land (r\land q)}}
% \def\lawEqvDef{\NmCmtLaw{$\equiv$-def}{$\GSN{3.52}$}{p \equiv q \equiv (p\land q) \lor (\lnot p \land \lnot q)}}
% \def\lawExor{\NmCmtLaw{exclusive-or}{$\GSN{3.53}$}{p\not \equiv q \equiv (\lnot p \land q) \lor (p\land \lnot q)}}
%
%
% % Implication

\def\CJweakenImp{P \land Q \implies P}
\def\CJweakenImpN{\QNAME{weaken-$\implies$}}

% \def\lawImpJoin{\NmCmtLaw{$\implies$-join}{$\GSN{3.57}$}{p \implies q \equiv p\lor q \equiv q}}
% \def\lawPmiDef{\NmCmtLaw{$\impliedby$-def}{$\GSN{3.58}$}{p \impliedby q \equiv q \implies p}}
% \def\lawImpDef{\NmCmtLaw{$\implies$-def}{$\GSN{3.59}$}{p\implies q \equiv \lnot p\lor q}}
% \def\lawImpMeet{\NmCmtLaw{$\implies$-meet}{$\GSN{3.60}$}{p\implies q \equiv p\land q\equiv p}}
% \def\lawContraPos{\NmCmtLaw{contrapositive}{$\GSN{3.61}$}{p\implies q \equiv \lnot q\implies \lnot p}}
% \def\lawImpEqvDistr{\NmCmtLaw{$\implies$-$\equiv$-distr}{$\GSN{3.63}$}{p \implies (q\equiv r) \equiv p\implies q \equiv p \implies r}}
% \def\lawShunting{\NmCmtLaw{shunting}{$\GSN{3.65}$}{p \land q\implies r \equiv p\implies (q \implies r)}}
% \def\lawAndImp{\NmCmtLaw{GS3.66}{$\GSN{3.66}$}{p \land (p\implies q) \equiv p\land q}}
% \def\lawAndPmi{\NmCmtLaw{GS3.67}{$\GSN{3.67}$}{p \land (q\implies p) \equiv p}}
% \def\lawOrImp{\NmCmtLaw{GS3.68}{$\GSN{3.68}$}{p \lor (p\implies q) \equiv \TRUE}}
% \def\lawOrPmi{\NmCmtLaw{GS3.69}{$\GSN{3.69}$}{p \lor (q\implies p) \equiv q\implies p}}
% \def\lawOrImpAnd{\NmCmtLaw{GS3.70}{$\GSN{3.70}$}{p \lor q\implies p\land q \equiv p \equiv q}}
% \def\lawImpRefl{\NmCmtLaw{$\implies$-refl}{$\GSN{3.71}$}{p\implies p \equiv \TRUE}}
% \def\lawImpRZero{\NmCmtLaw{$\implies$-r-zero}{$\GSN{3.72}$}{p \implies \TRUE \equiv \TRUE}}
% \def\lawImpLUnit{\NmCmtLaw{$\implies$-l-unit}{$\GSN{3.73}$}{\TRUE \implies p \equiv p}}
% \def\lawNotDef{\NmCmtLaw{$\lnot$-def}{$\GSN{3.74}$}{p\implies \FALSE \equiv \lnot p}}
% \def\lawFalseImp{\NmCmtLaw{GS3.75}{$\GSN{3.75}$}{\FALSE \implies p \equiv \TRUE}}
% \def\lawImpTrans{\NmCmtLaw{$\implies$-trans}{$\GSN{3.82}$}{(p\implies q)\land (q \implies r) \implies (p\implies r)}}
% \def\lawEqvImpTrans{\NmCmtLaw{$\equiv$-$\implies$-trans}{$\GSN{3.82}$}{(p\equiv q)\land (q \implies r) \implies (p\implies r)}}
% \def\lawImpEqvTrans{\NmCmtLaw{$\implies$-$\equiv$-trans}{$\GSN{3.82}$}{(p\implies q)\land (q \equiv r) \implies (p\implies r)}}
%
% \def\lawAnteStrngthn{
%   P \land Q \implies P
% }
% \def\lawCnsqWkn{
%   P \implies P \lor Q
% }
% \def\lawAnteOrDistr{
%   P \lor Q \implies R \quad\equiv\quad   (P \implies R)  \land (Q \implies R)
% }
% \def\lawAnteAndDistr{
%   P \land Q \implies R \quad\equiv\quad   (P \implies R)  \lor (Q \implies R)
% }
% \def\lawCnsqAndDistr{
%   P \implies Q \land R \quad\equiv\quad (P \implies Q) \land (P \implies R)
% }
% \def\lawCnsqOrDistr{
%   P \implies Q \lor R \quad\equiv\quad (P \implies Q) \lor (P \implies R)
% }
%
% %Equivalence and TRUE
% \def\lawEqvAssoc{\NmCmtLaw{$\equiv$-assoc}{$\GSN{3.1}$}{((p\equiv q)\equiv r) \equiv (p\equiv (q\equiv r))}}
% \def\lawEqvComm{\NmCmtLaw{$\equiv$-comm}{$\GSN{3.2}$}{p\equiv q \equiv q \equiv p}}
% \def\lawEqvUnit{\NmCmtLaw{$\equiv$-unit}{$\GSN{3.3}$}{\TRUE \equiv q \equiv q}}
% \def\lawTrue{\NmCmtLaw{true}{$\GSN{3.4}$}{\TRUE}}
% \def\lawEqvRefl{\NmCmtLaw{$\equiv$-refl}{$\GSN{3.5}$}{p\equiv p}}


\def\CONJPROP{
  \begin{array}{ll}
       \CJeqvId & \CJeqvIdN
    \\ \CJorZero & \CJorZeroN
    \\ \CJweakenImp & \CJweakenImpN
  \end{array}
}




%%%%  ==== Predicates ==========================================================

%% ---- Predicate Axioms -------------------------------------------------------

\def\AXorAllOScopeL{p \lor (\forall \lst x,\lst y @ q)}
\def\AXorAllOScopeR{\forall \lst x @ p \lor (\forall \lst y @ q)}
\def\AXorAllOScopeS{\lst x \notin p}
\def\AXorAllOScopeN{\QNAME{$\lor$-$\forall x$-scope}}
\def\AXorAllOScope{\AXorAllOScopeL \equiv \AXorAllOScopeR, \quad \AXorAllOScopeS}

\def\AXorAllEScopeL{p \lor (\forall \lst E, \lst F @ q)}
\def\AXorAllEScopeR{\forall \lst E @ p \lor (\forall \lst F @ q)}
\def\AXorAllEScopeS{\lst E \notin p}
\def\AXorAllEScopeN{\QNAME{$\lor$-$\forall E$-scope}}
\def\AXorAllEScope{\AXorAllEScopeL \equiv \AXorAllEScopeR, \quad \AXorAllEScopeS}

\def\AXorAllPScopeL{p \lor (\forall \lst P,  \lst Q @ q)}
\def\AXorAllPScopeR{\forall \lst P @ p \lor (\forall \lst Q @ q)}
\def\AXorAllPScopeS{ \lst P \notin p}
\def\AXorAllPScopeN{\QNAME{$\lor$-$\forall P$-scope}}
\def\AXorAllPScope{\AXorAllPScopeL \equiv \AXorAllPScopeR, \quad \AXorAllPScopeS}

\def\AXallODistrL{(\forall \lst x @ p \land q)}
\def\AXallODistrR{(\forall \lst x @ p) \land (\forall \lst x @ q)}
\def\AXallODistrN{\QNAME{$\forall x$-distr}}
\def\AXallODistr{\AXallODistrL \equiv \AXallODistrR}

\def\AXallEDistrL{(\forall \lst E @ p \land q)}
\def\AXallEDistrR{(\forall \lst E @ p) \land (\forall \lst E @ q)}
\def\AXallEDistrN{\QNAME{$\forall E$-distr}}
\def\AXallEDistr{\AXallEDistrL \equiv \AXallEDistrR}

\def\AXallPDistrL{(\forall \lst P @ p \land q)}
\def\AXallPDistrR{(\forall \lst P @ p) \land (\forall \lst P @ q)}
\def\AXallPDistrN{\QNAME{$\forall P$-distr}}
\def\AXallPDistr{\AXallPDistrL \equiv \AXallPDistrR}

\def\AXallOInstL{\forall x, \lst x @ p}
\def\AXallOInstR{\forall \lst x  @ p[e/x]}
\def\AXallOInstN{\QNAME{$\forall x$-inst}}
\def\AXallOInst{(\AXallOInstL) \implies (\AXallOInstR)}

\def\AXallEInstL{\forall E , \lst E @ p}
\def\AXallEInstR{\forall \lst E @ p[e/E]}
\def\AXallEInstN{\QNAME{$\forall E$-inst}}
\def\AXallEInst{(\AXallEInstL) \implies (\AXallEInstR)}

\def\AXallPInstL{\forall P, \lst P @ q}
\def\AXallPInstR{\forall \lst P @ q[r/P]}
\def\AXallPInstN{\QNAME{$\forall P$-inst}}
\def\AXallPInst{(\AXallPInstL) \implies (\AXallPInstR)}

\def\AXallORngL{\forall \lst x | r @ p}
\def\AXallORngR{\forall \lst x @ r \implies p}
\def\AXallORngN{\QNAME{$\forall x$-range}}
\def\AXallORng{(\AXallORngL) \equiv (\AXallORngR)}

\def\AXanyODefL{\exists \lst x @ p}
\def\AXanyODefR{\lnot (\forall \lst x @ \lnot p)}
\def\AXanyODefN{\QNAME{$\exists x$-def}}
\def\AXanyODef{(\AXanyODefL) \equiv \AXanyODefR}

\def\AXanyEDefL{\exists \lst E @ p}
\def\AXanyEDefR{\lnot (\forall \lst E @ \lnot p)}
\def\AXanyEDefN{\QNAME{$\exists E$-def}}
\def\AXanyEDef{(\AXanyEDefL) \equiv \AXanyEDefR}

\def\AXanyPDefL{\exists \lst P @ p}
\def\AXanyPDefR{\lnot (\forall \lst P @ \lnot p)}
\def\AXanyPDefN{\QNAME{$\exists P$-def}}
\def\AXanyPDef{(\AXanyPDefL) \equiv \AXanyPDefR}

\def\AXanyORngL{\exists \lst x | r @ p}
\def\AXanyORngR{\exists \lst x @ r \land p}
\def\AXanyORngN{\QNAME{$\exists x$-range}}
\def\AXanyORng{(\AXanyORngL) \equiv (\AXanyORngR)}

\def\AXoneODefL{\exists! \lst x @ p}
\def\AXoneODefR{(\exists \lst x @ p)
                 \land
                 \exists \lst y @ p[\lst y/ \lst x] \implies \lst y = \lst x}
\def\AXoneODefN{\QNAME{$\exists! x$-def}}
\def\AXoneODef{(\AXoneODefL) \equiv (\AXoneODefR)}

\def\AXoneORngL{\exists! \lst x | r @ p}
\def\AXoneORngR{\exists! \lst x @ r \land p}
\def\AXoneORngN{\QNAME{$\exists! x$-range}}
\def\AXoneORng{(\AXoneORngL) \equiv (\AXoneORngR)}

\def\AXunivClosureL{[p]}
\def\AXunivClosureR{\forall \lst x @ p}
\def\AXunivClosureS{\lst x \supseteq p}
\def\AXunivClosureN{\QNAME{$[]$-def}}
\def\AXunivClosure{\AXunivClosureL \equiv (\AXunivClosureR), \quad \AXunivClosureS}

\def\AXoneODefL{\exists! \lst x @ p}
\def\AXoneODefR{(\exists \lst x @ p)
                 \land
                 \exists \lst y @ p[\lst y/ \lst x] \implies \lst y = \lst x}
\def\AXoneODefN{\QNAME{$\exists! x$-def}}
\def\AXoneODef{(\AXoneODefL) \equiv (\AXoneODefR)}

\def\AXeqReflL{e}
\def\AXeqReflR{e}
\def\AXeqReflN{\QNAME{$=$-refl}}
\def\AXeqRefl{\AXeqReflL = \AXeqReflR}

\def\AXtheDefL{e=\theta x @ p}
\def\AXtheDefR{p[e/x] \land (\forall y @ p[y/x] \implies y=e)}
\def\AXtheDefS{x \notin e}
\def\AXtheDefN{\QNAME{$\theta$-Def}}
\def\AXtheDef{(\AXtheDefL) \equiv \AXtheDefR, \quad \AXtheDefS}

\def\AXtheRngL{\theta x | r @ p}
\def\AXtheRngR{\theta x @ r \land p}
\def\AXtheRngN{\QNAME{$\theta$-range}}
\def\AXtheRng{(\AXtheRngL) = (\AXtheRngR)}

\def\AXObetaRedL{(\lambda x, \lst x @ e)f}
\def\AXObetaRedR{(\lambda , \lst x @ e)[f/x]}
\def\AXObetaRedN{\QNAME{$\beta$-OReduce}}
\def\AXObetaRed{\AXObetaRedL = \AXObetaRedR}

\def\AXEbetaRedL{(\Lambda E, \lst E @ q)e}
\def\AXEbetaRedR{(\Lambda , \lst E @ q)[e/E]}
\def\AXEbetaRedN{\QNAME{$\beta$-EReduce}}
\def\AXEbetaRed{\AXEbetaRedL \equiv \AXEbetaRedR}

\def\AXPbetaRedL{(\Lambda P, \lst P @ q)r}
\def\AXPbetaRedR{(\Lambda , \lst P @ q)[r/P]}
\def\AXPbetaRedN{\QNAME{$\beta$-PReduce}}
\def\AXPbetaRed{\AXPbetaRedL \equiv \AXPbetaRedR}

\def\AXLeibnizL{\bigwedge_{i=1}^n x_i = e_i}
\def\AXLeibnizR{p \equiv p[\vec e/\vec x]}
\def\AXLeibnizS{x_i \mbox{ distinct}}
\def\AXLeibnizN{\QNAME{Leibniz}}
\def\AXLeibniz{(\AXLeibnizL) \implies (\AXLeibnizR), \quad \AXLeibnizS}

\def\AXLLeibnizL{\lst x = \lst e}
\def\AXLLeibnizR{p \equiv p[\lstvec e/\lstvec x]}
\def\AXLLeibnizN{\QNAME{LLeibniz}}
\def\AXLLeibniz{(\AXLLeibnizL) \implies (\AXLLeibnizR)}

\def\AXOSubstL{p[\vec e/\vec x]}
\def\AXOSubstR{p[\vec x:=\vec e]}
\def\AXOSubstN{\QNAME{OSubst}}
\def\AXOSubst{\AXOSubstL \equiv \AXOSubstR}

\def\AXESubstL{p[\vec e/\vec E]}
\def\AXESubstR{p[\vec E:=\vec e]}
\def\AXESubstN{\QNAME{ESubst}}
\def\AXESubst{\AXESubstL \equiv \AXESubstR}

\def\AXPSubstL{p[\vec q/ \vec P]}
\def\AXPSubstR{p[ \vec P:=\vec q]}
\def\AXPSubstN{\QNAME{PSubst}}
\def\AXPSubst{\AXPSubstL \equiv \AXPSubstR}

\def\AXTrueOSubL{true[\lst e/ \lst x]}
\def\AXTrueOSubR{true}
\def\AXTrueOSubN{\QNAME{$true$-OSubst}}
\def\AXTrueOSub{\AXTrueOSubL \equiv \AXTrueOSubR}

\def\AXTrueESubL{true[\lst e/ \lst E]}
\def\AXTrueESubR{true}
\def\AXTrueESubN{\QNAME{$true$-ESubst}}
\def\AXTrueESub{\AXTrueESubL \equiv \AXTrueESubR}

\def\AXTruePSubL{true[\lst q/ \lst P]}
\def\AXTruePSubR{true}
\def\AXTruePSubN{\QNAME{$true$-PSubst}}
\def\AXTruePSub{\AXTruePSubL \equiv \AXTruePSubR}

\def\AXFalseOSubL{false[\lst e/ \lst x]}
\def\AXFalseOSubR{false}
\def\AXFalseOSubN{\QNAME{$false$-OSubst}}
\def\AXFalseOSub{\AXFalseOSubL \equiv \AXFalseOSubR}

\def\AXFalseESubL{false[\lst e/ \lst E]}
\def\AXFalseESubR{false}
\def\AXFalseESubN{\QNAME{$false$-ESubst}}
\def\AXFalseESub{\AXFalseESubL \equiv \AXFalseESubR}

\def\AXFalsePSubL{false[\lst q/ \lst P]}
\def\AXFalsePSubR{false}
\def\AXFalsePSubN{\QNAME{$false$-PSubst}}
\def\AXFalsePSub{\AXFalsePSubL \equiv \AXFalsePSubR}

\def\AXNONPROP{
  \begin{array}{ll}
     \AXorAllOScopeL & \AXorAllOScopeN
  \\ {}\equiv (\AXorAllOScopeR), \quad \AXorAllOScopeS
  \\ \AXorAllEScopeL & \AXorAllEScopeN
  \\ {}\equiv (\AXorAllEScopeR), \quad \AXorAllEScopeS
  \\ \AXorAllPScopeL & \AXorAllPScopeN
  \\ {}\equiv (\AXorAllPScopeR), \quad \AXorAllPScopeS
  \\
  \\ \AXallODistr & \AXallODistrN
  \\ \AXallEDistr & \AXallEDistrN
  \\ \AXallPDistr & \AXallPDistrN
  \\
  \\ \AXallOInst & \AXallOInstN
  \\ \AXallEInst & \AXallEInstN
  \\ \AXallPInst & \AXallPInstN
  %\\ \AXallORng  & \AXallORngN
  \\
  \\ \AXanyODef & \AXanyODefN
  \\ \AXanyEDef & \AXanyEDefN
  \\ \AXanyPDef & \AXanyPDefN
  %\\ \AXanyORng & \AXanyORngN
  \\ \AXoneODefL & \AXoneODefN
  \\ {}\equiv \AXoneODefR
  \\ \AXunivClosure & \AXunivClosureN
   %\\ \AXoneORng & \AXoneORngN
  \\
  \\\AXeqRefl & \AXeqReflN
  %
  \\ (\AXtheDefL) & \AXtheDefN
  \\ {} \equiv \AXtheDefR,~\AXtheDefS
  %\\ \AXtheRng & \AXtheRngN
  %
  \\
  \\ \AXObetaRed & \AXObetaRedN
  \\ \AXEbetaRed & \AXEbetaRedN
  \\ \AXPbetaRed & \AXPbetaRedN
  %
  \\
  \\ \AXLeibniz, & \AXLeibnizN
  \\ \AXLeibnizS
  \\
  \\ \AXOSubst & \AXOSubstN
  \\ \AXESubst & \AXESubstN
  \\ \AXPSubst & \AXPSubstN
  \\ \AXTrueOSub & \AXTrueOSubN
  \\ \AXTrueESub & \AXTrueESubN
  \\ \AXTruePSub & \AXTruePSubN
  \\ \AXFalseOSub & \AXFalseOSubN
  \\ \AXFalseESub & \AXFalseESubN
  \\ \AXFalsePSub & \AXFalsePSubN
  \end{array}
}




%%%%  ==== Inference Rules =====================================================


\def\INFERENCES{
  \begin{array}{ll}
     \INFER{P}{P[Q:=R]}
   & \mbox{(Substitution)}
  \\
  \\ \INFER{P\equiv Q}{R[S:=P] \equiv R[S:=Q]}
   & \mbox{(Leibniz)}
  \\
  \\ \INFER{P, P \equiv Q}{Q}
   & \mbox{(Equanimity)}
  \end{array}
}




%%%%  ==== Strategies ==========================================================

\def\DERIVED{
\begin{array}{ll}
   \INFER{P\equiv Q , Q \equiv R}{P \equiv R}
 & \mbox{(Transitivity)}
%
\\ \Gamma \vdash p
   \quad\mbox{iff}\quad
   \Gamma \vdash p \equiv True
 & \mbox{(Truth-is-True)}
%
\\\hline\vspace{-9pt}
\\ \vdash (\forall\vec x,\lstvec q @ True) \equiv True
& \mbox{(Always-True)}
\\ \vdash (\forall \lst E @ True) \equiv True
\\ \vdash (\forall \lst P @ True) \equiv True
%
\\\hline\vspace{-9pt}
\\ \Gamma \vdash p
   \quad\mbox{iff}\quad
    \Gamma \vdash \forall\vec x,\lstvec q @ p
 & \mbox{($\forall$ Intro/Elim)}
\\ \Gamma \vdash p
   \quad\mbox{iff}\quad
    \Gamma \vdash \forall \lst E @ p
\\ \Gamma \vdash p
   \quad\mbox{iff}\quad
    \Gamma \vdash \forall \lst P @ p
%
\\\hline\vspace{-9pt}
\\ p \vdash \forall\vec x,\lstvec q @ p
 & \mbox{(Generalization)}
\\ p \vdash \forall \lst E @ p
 & p \vdash \forall \lst P @ p
%
\\\hline\vspace{-9pt}
\\ p \vdash p[\vec x:=\vec e]
 & \mbox{(Corr. Generalization)}
\\ p \vdash p[\lst E:=\vec e]
 & p \vdash p[ \lst P:=\lstvec q]
%
\\\hline\vspace{-9pt}
\\ \vdash p \implies (\forall\vec x,\vec y,\lstvec q @ r)
 & \mbox{(Universal Consequent 1)}
\\ \quad \equiv
          (\forall\vec x @ p \implies \forall\vec y,\lstvec q @ r),
          \quad \vec x \notin p
\\ \vdash p \implies (\forall \lst E,\lst E @ r)
\\ \quad \equiv
          (\forall \lst E @ p \implies \forall \lst E @ r),
          \quad \lst E \notin p
\\ \vdash p \implies (\forall \lst P, \lst Q @ r)
\\ \quad \equiv
          (\forall \lst P @ p \implies \forall \lst Q @ r),
          \quad  \lst P \notin p
%
\\\hline\vspace{-9pt}
\\ \vdash p \equiv \forall\vec x @ p,
   \quad \vec x \notin p
 & \mbox{(Corr. Univ. Conseq. 1)}
\\ \vdash p \equiv \forall \lst E @ p,
   \quad \lst E \notin p
 & \vdash p \equiv \forall \lst P @ p,
   \quad  \lst P \notin p
%
\\\hline\vspace{-9pt}
\\ \Gamma \vdash p \implies q
   \quad\mbox{iff}\quad
   \Gamma \vdash p \implies \forall\vec x @ q,
   \quad \vec x\notin p
 & \mbox{(Universal Consequent 2)}
\\ \Gamma \vdash p \implies q
   \quad\mbox{iff}\quad
   \Gamma \vdash p \implies \forall \lst E @ q,
   \quad \lst E\notin p
\\ \Gamma \vdash p \implies q
   \quad\mbox{iff}\quad
   \Gamma \vdash p \implies \forall \lst P @ q,
   \quad  \lst P\notin p
%
\\\hline\vspace{-9pt}
\\ \Gamma \vdash q \implies p
   \quad\mbox{iff}\quad
   \Gamma \vdash (\exists \vec x  @ q) \implies p,
   \quad \vec x\notin p
 & \mbox{(Corr. Univ.l Conseq. 2)}
\\ \Gamma \vdash q \implies p
   \quad\mbox{iff}\quad
   \Gamma \vdash (\exists \lst E  @ q) \implies p,
   \quad \lst E\notin p
\\ \Gamma \vdash q \implies p
   \quad\mbox{iff}\quad
   \Gamma \vdash (\exists  \lst P  @ q) \implies p,
   \quad  \lst P\notin p
%
\\\hline\vspace{-9pt}
\\ \vdash (\forall\vec x @ p) \equiv (\forall\vec z @ p[\vec x:=\vec z]),
   \quad \vec z \mbox{ fresh}
 & \mbox{($\alpha$-Renaming)}
\\ \vdash (\forall \lst E @ p) \equiv (\forall \lst F @ p[\lst E:=\lst F]),
   \quad \lst F \mbox{ fresh}
\\ \vdash (\forall \lst P @ p) \equiv (\forall \lst Q @ p[ \lst P:= \lst Q]),
   \quad  \lst Q \mbox{ fresh}
  \end{array}
}

\def\DEDUCTION{
  \begin{array}{ll}
     \Gamma, p \vdash q
     \quad\mbox{then}\quad
     \Gamma \vdash p \implies q,
     \quad p \mbox{ closed}
   & \mbox{(Deduction Theorem)}
  \\ \Gamma \vdash p \implies q
     \quad\mbox{then}\quad
     \Gamma, p \vdash q
   & \mbox{(Deduc. Converse)}
  \\ \Gamma, p[\vec x:=\vec k] \vdash q[\vec x:=\vec k]
     \quad\mbox{then}\quad
     \Gamma \vdash p \implies q,
   & \mbox{(Flexible Deduction)}
  \\\quad \vec x = \fv~p, \vec k \mbox{ constants.}
  \end{array}
}
